証明を追加した。

math/ssr_two_fib_eq.v
@@ -30,29 +30,48 @@ Section Two_Fib_Eq.
     | (m.+1 as pn).+1 => fib'1 m + fib'1 pn (* fib' n.-2 + fib' n.-1 *)
     end.
 
-  Fixpoint loop m n k :=
+  Fixpoint loop' m n k :=
     match k with
     | 0 => n
-    | k.+1 => loop n (n + m) k
+    | k.+1 => loop' n (n + m) k
     end.
-  Definition fib'2 n := loop 0 1 n.
+  Definition fib'2 n := loop' 0 1 n.
 
   Compute fib'1 5.                           (* 8 *)
   Compute fib'2 5.                           (* 8 *)
   
 (**
 ## idris の証明に近いもの
+
+- 補題
+loopIsLikeFib : (i, j, n: Nat) -> loop (i + j) (i + j + j) n = (loop j (i + j) n) + (loop i j n)
+loopIsLikeFib i j Z     = Refl
+loopIsLikeFib i j (S k) =
+  rewrite plusCommutative i j in
+  rewrite plusCommutative (j + i) j in
+  rewrite loopIsLikeFib j (j + i) k in
+  Refl
+
+-- 証明
+twoFibEq : (n: Nat) -> fib2 n = fib1 n
+twoFibEq Z         = Refl
+twoFibEq (S Z)     = Refl
+twoFibEq (S (S k)) =
+  rewrite loopIsLikeFib 0 1 k in
+  rewrite twoFibEq k in
+  rewrite twoFibEq (S k) in
+  Refl
 *)
-  Lemma loop_is_like_fib' i j n :
-    loop (i + j) (i + j + j) n = loop j (i + j) n + loop i j n.
+  Lemma loop'_is_like_fib' i j n :
+    loop' (i + j) (i + j + j) n = loop' j (i + j) n + loop' i j n.
   Proof.
     elim: n i j.
     - move=> i j.
       reflexivity.
     - move=> //= n IHn i j.
       Check IHn j (j + i)
-        : loop (j + (j + i)) (j + (j + i) + (j + i)) n =
-          loop (j + i) (j + (j + i)) n + loop j (j + i) n.
+        : loop' (j + (j + i)) (j + (j + i) + (j + i)) n =
+          loop' (j + i) (j + (j + i)) n + loop' j (j + i) n.
       rewrite [i + j]addnC.
       rewrite -[j + i + j]addnA [i + j]addnC.
       rewrite (IHn j (j + i)).
@@ -69,9 +88,9 @@ Section Two_Fib_Eq.
     (* fib'2 m.+2 = fib'1 m + fib'1 m.+1 *)
     - rewrite /fib'2 [LHS]/=.
       rewrite [1 + 0]addnC.
-      Check loop_is_like_fib' 0 1 m
-        : loop (0 + 1) (0 + 1 + 1) m = loop 1 (0 + 1) m + loop 0 1 m.
-      rewrite (loop_is_like_fib' 0 1 m).
+      Check loop'_is_like_fib' 0 1 m
+        : loop' (0 + 1) (0 + 1 + 1) m = loop' 1 (0 + 1) m + loop' 0 1 m.
+      rewrite (loop'_is_like_fib' 0 1 m).
       rewrite -IHn0.
       rewrite -IHn1.
       rewrite /fib'2 [RHS]/=.
@@ -82,8 +101,70 @@ Section Two_Fib_Eq.
 (**
 ## Coq風の証明
 *)  
+  Lemma loop'_is_like_fib i j n :
+    loop' (i + j) (i + j + j) n = loop' j (i + j) n + loop' i j n.
+  Proof.
+    elim: n i j => //= n IHn i j.
+    rewrite [i + j]addnC.
+    rewrite -[j + i + j]addnA [i + j]addnC.
+      by rewrite (IHn j (j + i)).
+  Qed.
+  
+  Theorem two_fib'_eq n : fib'2 n = fib'1 n.
+  Proof.
+    functional induction (fib'1 n) => //.
+    rewrite /fib'2 [LHS]/=.
+    rewrite (loop'_is_like_fib 0 1 m).
+    rewrite -IHn0.
+    rewrite -IHn1.
+    rewrite /fib'2 [RHS]/=.
+      by rewrite add0n addn0 [RHS]addnC.
+  Qed.
 
+(**
+# ふつうの fib の定義
+ *)
+  Function fib1 (n : nat) : nat :=
+    match n with
+    | 0 => 0
+    | 1 => 1
+    | (m.+1 as pn).+1 => fib1 m + fib1 pn (* fib n.-2 + fib n.-1 *)
+    end.
 
+  Fixpoint loop m n k :=
+    match k with
+    | 0 => m
+    | k.+1 => loop n (n + m) k
+    end.
+  Definition fib2 n := loop 0 1 n.
 
+  Compute fib1 5.                           (* 5 *)
+  Compute fib1 10.                          (* 55 *)
+  Compute fib2 5.                           (* 5 *)
+  Compute fib2 10.                          (* 5 *)
 
+  
+  Lemma loop_is_like_fib i j n :
+    loop (i + j) (i + j + j) n = loop j (i + j) n + loop i j n.
+  Proof.
+    elim: n i j => //= [| n IHn] i j.
+    - by rewrite addnC.
+    - rewrite [i + j]addnC.
+      rewrite -[j + i + j]addnA [i + j]addnC.
+      by rewrite (IHn j (j + i)).
+  Qed.
+  
+  Theorem two_fib_eq n : fib2 n = fib1 n.
+  Proof.
+    functional induction (fib1 n) => //.
+    rewrite /fib2 [LHS]/=.
+    rewrite (loop_is_like_fib 0 1 m).
+    rewrite -IHn0.
+    rewrite -IHn1.
+    rewrite /fib2 [RHS]/=.
+      by rewrite add0n addn0 [RHS]addnC.
+  Qed.
 
+End Two_Fib_Eq.
+
+(* END *)
